Able to prove some more important facts for `all_scmra`

new/experiments/all_scmra.v
@@ -36,196 +36,7 @@ End cmra_expr.
 Section defn.
 Context (Σ : gFunctors).
 
-(* This would require ucmra for everything, which would exclude exclR. *)
 Definition any_cmra : Type := discrete_funUR (optionUR ∘ cmra_expr.interpret Σ).
-
-(*
-Inductive csigT {A : Type} P :=
-| CexistT : ∀ (x : A), P x → csigT P
-| Cinvalid : csigT P.
-Global Arguments CexistT {_ _} (_).
-Global Arguments Cinvalid {_ _}.
-
-Definition any_cmra Σ : Type := csigT (cmra_expr.interpret Σ).
-
-Inductive any_cmra_equiv_instance : Equiv (any_cmra Σ) :=
-| CexistT_equiv {A} a b : a ≡ b → (CexistT A a) ≡ (CexistT A b)
-| Cinvalid_equiv : Cinvalid ≡ Cinvalid.
-Local Existing Instance any_cmra_equiv_instance.
-
-Inductive any_cmra_dist_instance : Dist (any_cmra Σ) :=
-| CexistT_dist {A} a b i : a ≡{i}≡ b → (CexistT A a) ≡{i}≡ (CexistT A b)
-| Cinvalid_dist i : Cinvalid ≡{i}≡ Cinvalid.
-Local Existing Instance any_cmra_dist_instance.
-
-Local Instance any_cmra_valid_instance : Valid (any_cmra Σ):=
-  λ x, match x with CexistT A a => ✓ a | _ => False end.
-
-Local Instance any_cmra_validN_instance : ValidN (any_cmra Σ) :=
-  λ n x, match x with CexistT A a => ✓{n} a | _ => False end.
-
-Local Instance any_cmra_pcore_instance : PCore (any_cmra Σ) :=
-  λ x, match x with CexistT A a => CexistT A <$> pcore a | _ => Some Cinvalid end.
-
-Local Instance any_cmra_op_instance : Op (any_cmra Σ) :=
-  λ x y,
-    match x, y with
-    | CexistT A a, CexistT A' a' =>
-        match (excluded_middle_informative (A = A')) with
-        | right _ => Cinvalid
-        | left eq_proof =>
-            CexistT A' ((eq_rect A (cmra_expr.interpret Σ) a A' eq_proof) ⋅ a')
-        end
-    | _, _ => Cinvalid
-    end.
-
-(* Q: does [inj_pair2] *require* [classical]? *)
-
-Local Instance any_cmra_dist_equivalence n : Equivalence (dist n (A:=any_cmra Σ)).
-split.
-+ intros ?. destruct x; constructor. apply reflexivity.
-+ intros ?? Heq. oinversion Heq; subst; constructor.
-  symmetry. done.
-+ intros ??? Heqy Heqz. oinversion Heqy; subst; oinversion Heqz; subst; constructor.
-  apply inj_pair2 in H4. subst. by etransitivity.
-Qed.
-
-Local Instance any_cmra_equiv_equivalence : Equivalence (equiv (A:=any_cmra Σ)).
-split.
-+ intros ?. destruct x; constructor. apply reflexivity.
-+ intros ?? Heq. oinversion Heq; subst; constructor.
-  symmetry. done.
-+ intros ??? Heqy Heqz. oinversion Heqy; subst; oinversion Heqz; subst; constructor.
-  apply inj_pair2 in H3. subst. by etransitivity.
-Qed.
-
-Lemma any_cmra_ofe_mixin : OfeMixin (any_cmra Σ).
-Proof.
-  split.
-  - intros; split.
-    + intros Heq n. inversion Heq; constructor. by apply equiv_dist.
-    + intros Heq. oinversion (Heq 0ᵢ); subst; constructor.
-      apply equiv_dist => n. oinversion (Heq n); subst.
-      apply inj_pair2 in H4, H5. subst. done.
-  - apply _.
-  - intros ???? Heq Hlt. oinversion Heq; constructor; subst.
-    by eapply dist_le.
-Qed.
-
-Lemma any_cmra_validN A a n :
-  ✓{n} CexistT A a ↔ ✓{n} a.
-Proof. done. Qed.
-
-Lemma any_cmra_valid A a :
-  ✓ CexistT A a ↔ ✓ a.
-Proof. done. Qed.
-
-Lemma any_cmra_invalid_validN n :
-  ✓{n} Cinvalid = False.
-Proof. done. Qed.
-
-Lemma any_cmra_invalid_valid :
-  ✓ Cinvalid = False.
-Proof. done. Qed.
-
-Lemma CexistT_op A a a' :
-  CexistT A a ⋅ CexistT A a' = CexistT A (a ⋅ a').
-Proof.
-  cbn. destruct excluded_middle_informative; try done. rewrite (UIP_refl _ _ e) //.
-Qed.
-
-Lemma any_cmra_included x y :
-  x ≼ y ↔ y = Cinvalid ∨ (∃ A a a', x = CexistT A a ∧ y = CexistT A a' ∧ a ≼ a').
-Proof.
-  split.
-  - intros [z Heq]. destruct y; last by left. right.
-    destruct x, z; cbn in *; try destruct excluded_middle_informative in Heq; subst; oinversion Heq.
-    subst. repeat eexists. apply inj_pair2 in H2, H4. subst. done.
-  - intros [|].
-    + subst. eexists Cinvalid. by destruct x.
-    + destruct H as (? & ? & ? & -> & -> & Hincl). destruct Hincl as [i Hincl].
-      eexists (CexistT x0 i). rewrite CexistT_op. constructor. done.
-Qed.
-
-Lemma any_cmra_cmra_mixin : CmraMixin (any_cmra Σ).
-Proof.
-  split.
-  - intros [] ? ? ? H.
-    + inversion H; subst; last done.
-      cbn. destruct excluded_middle_informative; constructor. rewrite H0 //.
-    + cbn. constructor.
-  - intros. oinversion H; subst; simpl.
-    + rewrite /pcore /any_cmra_pcore_instance in H0 |- *.
-      apply fmap_Some_1 in H0 as [? [Hpcore ?]]; subst.
-      eapply cmra_pcore_ne in Hpcore; last eassumption.
-      destruct Hpcore as (ca & -> & Heq).
-      eexists _; split; first done. constructor. done.
-    + eexists _. split; done.
-  - intros ?. intros ?? Heq. inversion Heq; last done.
-    rewrite !any_cmra_validN. by apply cmra_validN_ne.
-  - pose 0ᵢ. intros [|].
-    + setoid_rewrite any_cmra_validN. rewrite /= any_cmra_valid ?cmra_valid_validN //.
-    + rewrite any_cmra_invalid_valid. split; try done.
-      intros H. specialize (H 0). done.
-  - intros n m [|]; simpl; eauto using cmra_validN_le.
-  - intros [|] [|] [|]; try constructor.
-    + cbn. repeat (destruct excluded_middle_informative; subst; cbn); try constructor; try congruence.
-      unfold eq_rect. rewrite (UIP_refl _ _ e). rewrite assoc //.
-    + cbn. repeat (destruct excluded_middle_informative; subst; cbn); try constructor; try congruence.
-  - intros [|] [|]; try constructor. cbn.
-    repeat (destruct excluded_middle_informative; subst; cbn); try constructor; try congruence.
-    rewrite (UIP_refl _ _ e). rewrite comm //.
-  - intros [? a|] ? [=]; subst; auto. cbn in *.
-    destruct (pcore a) as [ca|] eqn:?; simplify_option_eq.
-    cbn. destruct excluded_middle_informative; try done.
-    constructor; rewrite (UIP_refl _ _ e). simpl. eauto using cmra_pcore_l.
-  - intros [? a|] ? [=]; subst; auto. cbn in *.
-    destruct (pcore a) as [ca|] eqn:?; simplify_option_eq. cbn.
-    oinversion (cmra_pcore_idemp a ca); repeat constructor; auto.
-  - intros ??? Hincl Hpcore. rewrite any_cmra_included in Hincl. destruct Hincl.
-    + subst. eexists Cinvalid. split; first done. eexists Cinvalid. destruct cx; reflexivity.
-    + destruct H as (? & ? & ? & -> & -> & Hincl). cbn in *. simplify_option_eq. rename H into p.
-      eapply cmra_pcore_mono in Hincl; try eassumption. destruct Hincl as (? & -> & Hincl).
-      destruct Hincl as [i Hincl]. eexists _. split; first done. eexists (CexistT x0 i).
-      cbn. destruct excluded_middle_informative; try done.
-      rewrite (UIP_refl _ _ e). simpl. constructor. done.
-  - intros n [|] [|]; simpl; try done.
-    cbn. destruct excluded_middle_informative; last done.
-    destruct e. simpl. cbn. eauto using cmra_validN_op_l.
-  - intros n [? a|] y1 y2 Hx Hx'.
-    + destruct y1 as [? a1|], y2 as [? a2|]; try by exfalso; inversion Hx'.
-      cbn in Hx'. destruct excluded_middle_informative in Hx'; last (exfalso; oinversion Hx').
-      subst. simpl in *. destruct (excluded_middle_informative (x = x1)).
-      2:{ exfalso. inversion Hx'. subst. done. }
-      subst.
-      destruct (cmra_extend n a a1 a2) as (z1&z2&?&?&?); [done| |].
-      * inversion Hx'. subst. apply inj_pair2 in H2, H3. subst. done.
-      * repeat econstructor; try done.
-        cbn. destruct excluded_middle_informative; last done.
-        rewrite (UIP_refl _ _ e). simpl. constructor. done.
-    + destruct y1 as [a1|], y2 as [a2|]; try by exfalso; inversion Hx'.
-Qed.
-
-Canonical Structure any_cmraO : ofe := Ofe (any_cmra Σ) any_cmra_ofe_mixin.
-Canonical Structure any_cmraR := Cmra (any_cmra Σ) any_cmra_cmra_mixin.
-
-Lemma any_cmra_validN_op A B a b n :
-  ✓{n} (CexistT A a ⋅ CexistT B b) ↔
-  ∃ (pf : A = B), ✓{n}((eq_rect A _ a B pf) ⋅ b).
-Proof.
-  split.
-  - intros H. cbn in H. destruct excluded_middle_informative in H; try done.
-    exists e. destruct e. simpl in *. rewrite any_cmra_validN // in H.
-  - intros (? & H). subst. simpl in *. rewrite CexistT_op //.
-Qed.
-
-Lemma any_cmra_validN_op_invalid_r A a n :
-  ✓{n} (CexistT A a ⋅ Cinvalid) → False.
-Proof. done. Qed.
-
-Lemma any_cmra_validN_op_invalid_l A a n :
-  ✓{n} (Cinvalid ⋅ CexistT A a) → False.
-Proof. done. Qed. *)
 
 Definition cast {A B : cmra} (a : A) (e : A = B) : B :=
   match e in (_ = A) return A with eq_refl => a end.
@@ -268,6 +79,8 @@ Proof.
   simpl. done.
 Qed.
 
+Definition any_cmraR Σ := discrete_funR (optionUR ∘ cmra_expr.interpret Σ).
+
 End defn.
 
 Section own.
@@ -280,7 +93,7 @@ Class SimpleCmra A :=
   }.
 
 Definition own_any {A : cmra} γ (a : A) : iProp Σ :=
-  ∃ (_ : SimpleCmra A), own γ (CexistT Aexp (eq_rect A id a _ eq_proof) : any_cmra Σ).
+  ∃ (_ : SimpleCmra A), own γ (to_any Σ Aexp (cast a eq_proof) : any_cmra Σ).
 
 Lemma own_any_update γ {A : cmra} (a a' : A) :
   a ~~> a' →
@@ -293,14 +106,39 @@ Proof.
   apply Hupd.
 Qed.
 
+Global Instance own_any_combine {A : cmra} γ (a b : A) :
+  CombineSepAs (own_any γ a) (own_any γ b) (own_any γ (a ⋅ b)).
+Proof.
+  rewrite /CombineSepAs. iIntros "[H1 H2]".
+  rewrite /own_any. iDestruct "H1" as "[% H1]".
+  iDestruct "H2" as "[% H2]". iExists _.
+  iCombine "H1 H2" as "H".
+  iExactEq "H". f_equal.
+  destruct H, H0. simpl in *.
+  unfold to_any.
+  apply FunctionalExtensionality.functional_extensionality_dep_good.
+  intros C. rewrite discrete_fun_lookup_op.
+  destruct excluded_middle_informative as [Heq|Hbad];
+    destruct excluded_middle_informative as [Heq'|Hbad'].
+  2:{ exfalso. apply Hbad'. rewrite -Heq. naive_solver. }
+  2:{ exfalso. apply Hbad. rewrite -Heq'. naive_solver. }
+  2:{ done. }
+  subst. simpl in *.
+  destruct Heq, Heq'. simpl in *.
+  pose proof (UIP_refl _ _ eq_proof1). subst. done.
+  (* FIXME: use [any_cmra_op] instead of manually proving? *)
+Qed.
+
 Lemma own_any_alloc `{!SimpleCmra A} (a : A) :
   ✓ a →
   ⊢ |==> ∃ γ, own_any γ a.
 Proof.
   intros Hvalid.
-  iMod (own_alloc (CexistT Aexp (eq_rect A id a _ eq_proof) : any_cmra Σ)) as (γ) "H".
-  { rewrite any_cmra_valid. simpl. destruct SimpleCmra0.
-    simpl in *. destruct eq_proof0. simpl in *. done. }
+  iMod (own_alloc (to_any Σ Aexp (eq_rect A id a _ eq_proof) : any_cmra Σ)) as (γ) "H".
+  { intros ?. rewrite /= /to_any.
+    destruct excluded_middle_informative as [Heq|Hbad]; last done.
+    destruct Heq. simpl in *. destruct SimpleCmra0.
+    subst. done. }
   by iFrame.
 Qed.
 
@@ -336,28 +174,6 @@ Lemma interpret_inj a a' :
   a = a'.
 Proof.
 Admitted.
-
-Global Instance own_any_combine {A : cmra} γ (a b : A) :
-  CombineSepAs (own_any γ a) (own_any γ b) (own_any γ (a ⋅ b)).
-Proof.
-  rewrite /CombineSepAs. iIntros "[H1 H2]".
-  rewrite /own_any. iDestruct "H1" as "[% H1]".
-  iDestruct "H2" as "[% H2]". iExists _.
-  iCombine "H1 H2" as "H".
-  iExactEq "H". f_equal.
-  destruct H, H0. subst.
-  simpl. pose proof (interpret_inj _ _ eq_proof1).
-  subst.
-  rewrite -is_op.
-
-  Search cmra_op.
-  rewrite is_op.
-  simpl.
-  rewrite
-  rewrite
-  constructor. sijkmpl.
-  intros ?.
-Qed.
 
 Section saved_pred.
 Context {A : Type}.
